Cleaned up imports.

coq/pcc/pcc4irm.v
@@ -1,226 +1,18 @@
-(* SS_Reflect tutorial: http://inria.ccsd.cnrs.fr/docs/00/25/94/78/PDF/RR-6455.pdf *)
 
-Require Import Bool.
-Require Import Omega.
-Require Import Wf.
-Require Import Wellfounded.
-Require Import ssreflect.
 Require Import list_utils.
-Require Import semantics_assertions.
-Require Import weakest_precondition.
-Require Import validity.
+Require Export validity.
+Require Export security_defs.
+Require Import ssreflect.
 
 
 
-
-
-
-
-(******************************************************************************)
-(*                                                                            *)
-(*    CONTRACTS                                                               *)
-(*                                                                            *)
-(******************************************************************************)
 Section contracts.
-  
-  Open Scope type_scope.
-  
-  Inductive event :=
-  | bef_event (_: classid) (_: methid) (arg: value)
-  | aft_event (_: classid) (_: methid) (ret: value)
-  | exc_event (_: classid) (_: methid).
-  
-  Definition event_trace := list event.
-  
-  (* The following definition is not distributive under ++ operations.
-     That is, trace_of (exec1 ++ exec2) <> (trace_of exec1) ++ (trace_of exec2) *)
-  Definition observed_event (p: program) (c: conf) : option event :=
-    match c with
-      | (gv, h, normal c m pc s ls :: ars) =>
-        match (instr_at p c m pc) with
-          | invoke c' m' => Some (bef_event c' m' (s[[0]]))
-          | ret => Some (aft_event c m (s[[0]]))
-          | _ => None
-        end
-      | (gv, h, exceptional o :: ars) => None (* add exc_event *)
-      | (gv, h, nil) => None
-    end.
-  
-  Fixpoint event_trace_of (p: program) (e: execution) : event_trace :=
-    match e with
-      | nil => nil
-      | c :: e' => match observed_event p c with
-                    | Some evt => evt :: event_trace_of p e'
-                    | None => event_trace_of p e'
-                  end
-    end.
-  
-  
-  Lemma event_trace_distr : forall p l l', event_trace_of p (l ++ l') =
-                                      event_trace_of p l ++ event_trace_of p l'.
-    intros.
-    induction l.
-    reflexivity.
-    rewrite <- app_comm_cons.
-    simpl.
-    destruct (observed_event p a).
-    rewrite IHl.
-    reflexivity.
-    rewrite IHl.
-    reflexivity.
-  Qed.
-  
-  
-  Inductive event_modifier := before | after  | exception.
-  
-  Definition contract := (event_modifier * classid * methid) -> ghost_update.
-  
-  Definition sec_state := ghost_valuation.
-  
-  Definition sec_state_trace := list sec_state.
-  
-  
-  Inductive ss_updates_of (contr : contract) : event_trace -> list ghost_update -> Prop :=
-  | ssu_done : ss_updates_of contr nil nil
-  | ssu_bef  : forall c m arg t' gus', ss_updates_of contr t' gus' ->
-                                  ss_updates_of contr (bef_event c m arg :: t') (contr (before, c, m) :: gus')
-  | ssu_aft  : forall c m ret t' gus', ss_updates_of contr t' gus' ->
-                                  ss_updates_of contr (aft_event c m ret :: t') (contr (after, c, m) :: gus').
-  
-  Inductive sst_tail : list ghost_update -> sec_state_trace -> Prop :=
-  | sst_done : forall ss, sst_tail nil (ss :: nil)
-  | sst_step : forall ss ss' gvar exp v sst gus, 
-        g_eeval exp ss v -> 
-        ss' = (upd_gv ss gvar v) ->
-        sst_tail gus (ss' :: sst) ->
-        sst_tail ((gvar, exp) :: gus) (ss :: ss' :: sst).
-  
-  Definition is_sec_state_trace (ssus : list ghost_update) (sst : sec_state_trace) : Prop :=
-    head sst = Some initial_gv /\ sst_tail ssus sst.
-  
-  
+
   (* For simplicity: The ghost state is represented by a single fixed ghost variable 'gs'. *)
   (* We still have a notion of ghost valuations to be able to handle local ghost variables
      used for storing arguments and return values. *)
   Variable gs : ghostid.
   
-  
-  Definition violating_sec_state (gv: ghost_valuation) := gv gs = ghost_errval.
-  
-  
-  Definition accepted_by contr (event_tr: event_trace) :=
-    forall gus sec_tr, 
-      ss_updates_of contr event_tr gus ->
-      is_sec_state_trace gus sec_tr ->
-      hd initial_gv sec_tr = initial_gv ->
-      (forall ss, In ss sec_tr -> ~ violating_sec_state ss).
-  
-  
-  Definition adheres_to p contr : Prop :=
-    forall `(execution_of p e), accepted_by contr (event_trace_of p e).
-  
-  
-  (*
-  The original definition of "Ghost Instruction Goes Wrong" is, 
-  "no guards of the ghost instruction hold".
-  If all inserted ghost instructions has the shape
-  
-    x := g_1 -> v_1 | g_2 -> v_2 | ... | g_n -> v_n | ghost_errval
-  
-  the notion of going wrong is equivalent to "no ghost var equals ghost_errval".
-  This is the reason why initial_gv has all vars initialized to 0 instead of ghost_errval.
-  *)
-  
-  
-  Definition exec_never_goes_wrong e :=
-    forall c, In c e -> ~ violating_sec_state (ghost_valuation_of c).
-  
-  
-  Section ghost_inliner.
-    
-    (* Note that assertions are irrelevant in this section. *)
-    
-    Variable contr: contract.
-    
-    (* My initial attempt encoded the ghost_inliner as a function. That approach
-       ran into the following problem:
-       
-       If a ghost instruction is to be inserted, it needs a label. Since method
-       bodies are total mappings from lables to instructions, it is impossible
-       to dig out a fresh label.
-       
-       The obvious fix would be to let method bodies be partial ("option")
-       mappings. Unfortunately the option-type spreads like a plague in the defs
-       and all proofs needs splitting on Some/None.
-       
-       This is why it is currently encoded as a proposition over programs. *)
-    
-    Definition ghost_inlined_meth (m gm: method) : Prop :=
-      forall l,
-        let l'   := label_function_of gm l in
-        let l''  := label_function_of gm l' in
-        let l''' := label_function_of gm l'' in
-          
-        forall (c: classid) (m': methid),
-          match minstr_at m l with
-          | invoke c m' => minstr_at gm l   = ghost_instr (contr (before, c, m')) /\
-                           minstr_at gm l'  = invoke c m' /\
-                           minstr_at gm l'' = ghost_instr (contr (after, c, m')) /\
-                           label_function_of m l = l'''
-          | i => minstr_at gm l = i /\
-                 label_function_of m l = l
-          end.
-    
-    
-    Definition ghost_inlined_class (c gc: class) : Prop :=
-      forall mid, ghost_inlined_meth (c mid) (gc mid).
-
-    Definition ghost_inlined (p pg: program) : Prop :=
-      forall cid, ghost_inlined_class (classes pg cid) (classes p cid).
-  
-  End ghost_inliner.
-  
-  (*
-  Definition ghost_update_of pg (c : conf) : option ghost_update :=
-    match c with
-      | (_, _, normal c m pc s l :: _) =>
-        match instr_at pg c m pc with
-          | ghost_instr gu => Some gu
-          | otherwise => None
-        end
-      | otherwise => None
-    end.
-  *)
-  Definition ghost_update_of pg (c : conf) : option ghost_update :=
-    match current_instr pg c with
-      | Some (ghost_instr gu) => Some gu
-      | _ => None
-    end.
-
-  (* Returns ghost updates that *have been carried out* (to be compatible with ss_after). *)
-  Fixpoint ghost_updates_of pg (eg : execution) : list ghost_update :=
-    match eg with
-      | nil => nil
-      | c :: eg' =>
-        match eg' with
-          | nil => nil
-          | c' :: eg'' =>
-            match ghost_update_of pg c with
-              | Some gu => gu :: ghost_updates_of pg eg'
-              | None => ghost_updates_of pg eg'
-            end
-        end
-    end.
-  
-  Fixpoint seen_ghost_updates_of pg (eg : execution) : list ghost_update :=
-    match eg with
-      | nil => nil
-      | c :: eg' =>
-        match ghost_update_of pg c with
-          | Some gu => gu :: seen_ghost_updates_of pg eg'
-          | None => seen_ghost_updates_of pg eg'
-        end
-    end.
   
   Lemma seen_ghost_updates_of_distr p :
     forall e1 e2, seen_ghost_updates_of p (e1 ++ e2) = seen_ghost_updates_of p e1 ++ seen_ghost_updates_of p e2. 
@@ -1164,8 +956,8 @@ Qed.
   Theorem never_wrong_impl_ghost_adherence p contr `(ghost_inlined contr p pg) :
     (forall eg,
       execution_of pg eg ->
-      exec_never_goes_wrong eg) ->
-    adheres_to pg contr.
+      exec_never_goes_wrong gs eg) ->
+    adheres_to gs pg contr.
   Proof.
     unfold adheres_to.
     unfold accepted_by.
@@ -1411,7 +1203,7 @@ Qed.
   Qed.
   
   Lemma ghost_adherence_impl_actual_adherence :
-    forall p contr, (exists pg, ghost_inlined contr p pg /\ adheres_to pg contr) -> adheres_to p contr.
+    forall p contr, (exists pg, ghost_inlined contr p pg /\ adheres_to gs pg contr) -> adheres_to gs p contr.
   Proof.
     intros p contr H.
     unfold adheres_to.
@@ -1433,8 +1225,8 @@ Qed.
   Corollary never_wrong_impl_adherence p contr :
     (exists pg,
       ghost_inlined contr p pg /\
-      forall `(execution_of pg gexec), exec_never_goes_wrong gexec) ->
-      adheres_to p contr.
+      forall `(execution_of pg gexec), exec_never_goes_wrong gs gexec) ->
+      adheres_to gs p contr.
   Proof.
     intros.
     elim H; intros pg H_gadh.
@@ -1488,9 +1280,9 @@ Qed.
 (* Lemma: only way to go from non-violating conf to violating conf is to execute a ghost instr with rhs evaluating to \bot *)
 Lemma non_vio_to_vio_impl_ghost_err :
   forall p c c',
-    ~ violating_sec_state (ghost_valuation_of c) ->
+    ~ violating_sec_state gs (ghost_valuation_of c) ->
     trans p c c' ->
-    violating_sec_state (ghost_valuation_of c') ->
+    violating_sec_state gs (ghost_valuation_of c') ->
     exists gexpr,
       current_instr p c = Some (ghost_instr (gs, gexpr)) /\
       g_eeval gexpr (ghost_valuation_of c) ghost_errval.
@@ -1580,7 +1372,7 @@ Qed.
   
   
   Lemma initial_not_violating :
-    forall c, initial_conf c -> ~ violating_sec_state (ghost_valuation_of c).
+    forall c, initial_conf c -> ~ violating_sec_state gs (ghost_valuation_of c).
   Proof.
     intros.
     intro.
@@ -1603,7 +1395,7 @@ Qed.
       label_function_of (classes pg c m) l = l' ->
       annotations_of (classes pg c m) l' = a ->
       stronger_ast a (neg (eq (ghost_var gs) ghost_errval))) ->
-    forall `(execution_of pg exec), exec_never_goes_wrong exec.
+    forall `(execution_of pg exec), exec_never_goes_wrong gs exec.
   Proof.
 intros.
 destruct exec using rev_ind.
@@ -1654,7 +1446,7 @@ apply sub_execution in H_exec.
 apply IHexec in H_exec.
 unfold exec_never_goes_wrong in H_exec.
 pose proof (H_exec c).
-assert (H_1 : ~ violating_sec_state (ghost_valuation_of c)).
+assert (H_1 : ~ violating_sec_state gs (ghost_valuation_of c)).
   apply H2; auto with datatypes.
 
 intro.
@@ -1866,7 +1658,7 @@ Qed.
   Theorem proof_outline_existence_impl_adherence :
     forall p contr,
       (exists annos, is_proof_outline p contr annos) ->
-      adheres_to p contr.
+      adheres_to gs p contr.
     Proof.
       intros.
       elim H; intros annos H_po.
